Transcribing the content of [square_abstraction.v] to [hypercube_abstraction.v]... pretty mechanical work... maybe I should do some more thinking/planning?...
darcs-hash:20100317170346-20b81-bd42d2e44196b1033a374b8c895075ee55388865.gz

hypercube_abstraction.v
@@ -67,8 +67,8 @@ Section contents.
     (intervals_range : forallDim (fun i ip => B (Vnth intervals ip) -> OpenQRange))
     (absInterval : forall (l : concrete.Location chs) (p : concrete.Point chs), concrete.invariant (l, p) ->
       forallDim (fun i ip =>
-        DN (sig (fun int : B (Vnth intervals ip) => in_orange (intervals_range i ip int) (Vnth (pxy p) ip))
-      ))).
+        DN { int : B (Vnth intervals ip) | in_orange (intervals_range i ip int) (Vnth (pxy p) ip)}
+    )).
 
   Definition ap_inv_DN :
     forall (i : nat) (ip : (i < n)%nat) (l : concrete.Location chs) (p : concrete.Point chs),
@@ -104,5 +104,169 @@ Section contents.
 
   For instance, we can easily make an invariant overestimator 
   (if one's invariant can be overestimated by a list of open squares): *)
+
+  Section invariant_overestimator.
+
+    Variable invariant_squares :
+      forall l : concrete.Location chs, 
+        { s : OpenHCube n | forall p, concrete.invariant (l, p) -> in_ohypercube (pxy p) s }.
+
+    Program Definition make_invariant_overestimator : overestimator (@abstract.invariant _ ap) := _.
+    Admit Obligations.
+(*      fun li => overestimate_osquares_overlap eps (invariant_squares (fst li)) (square (snd li)).*)
+
+  End invariant_overestimator.
+
+  (* Similarly, if one's initial condition can be overestimated by
+   an open square, we can make an initial_dec thingy. *)
+
+  Section make_initial_overestimator.
+
+    Variables
+      (initial_location : concrete.Location chs)
+      (initial_square : OpenHCube n)
+      (initial_representative : forall s, concrete.initial s ->
+        fst s = initial_location /\ in_ohypercube (pxy (snd s)) initial_square).
+
+    Program Definition make_initial_overestimator (eps : Qpos) : overestimator (@abstract.Initial _ ap) := 
+      fun s => _.
+    Admit Obligations.
+(*
+        (overestimate_conj (overestimate_osquares_overlap eps (initial_square) (square (snd s)))
+          (decision_overestimation (concrete.Location_eq_dec chs (fst s) initial_location))).
+*)
+
+  End make_initial_overestimator. 
   
+  (* And similarly, if one's guard conditions can be overestimated by
+  open squares, we can make a guard_dec thingy. *)
+
+  Section make_guard_overestimator.
+
+    Definition GuardSquare l l' := 
+      { s : option (OpenHCube n) | forall p, concrete.guard chs (l, p) l' ->
+          match s with
+          | None => False
+          | Some v => in_ohypercube (pxy p) v
+          end
+      }.
+
+    Program Definition guard_dec (guard_square : forall l l', GuardSquare l l') (eps : Qpos) : 
+      overestimator (@abstract.guard _ ap) := 
+      _.
+    Admit Obligations.
+(*
+      fun l r l' =>
+      match guard_square l l' with
+      | Some s => overestimate_osquares_overlap eps s (square r)
+      | None => false
+      end.
+*)
+
+  End make_guard_overestimator.  
+
+  (* If the safety condition can be overestimated by a list of unsafe
+   osquares, then we can select the unsafe abstract states automatically: *)
+
+  Section square_safety.
+
+    Variables
+      (unsafe_concrete : concrete.State chs -> Prop)
+      (unsafe_squares : concrete.Location chs -> list (OpenHCube n))
+      (unsafe_squares_correct: forall s, unsafe_concrete s -> exists q,
+        In q (unsafe_squares (fst s)) /\ in_ohypercube (pxy (snd s)) q)
+      (eps: Qpos).
+
+      Program Definition unsafe_abstract : abstract.CompleteCoverList ap unsafe_concrete :=
+        _.
+(*
+      := flat_map (fun l => map (pair l) (flat_map (fun q =>
+        filter (fun s => overestimate_osquares_overlap eps q (square s)) exhaustive_list
+        ) (unsafe_squares l))) (concrete.locations chs).
+*)
+      Admit Obligations.
+
+  End square_safety.
+
+  (* Everything above is pretty simplistic. We now prepare for more complex
+   transition overestimators, for which we will require some more stuff: *)
+
+  Let reset_function := concrete.Location chs -> concrete.Location chs -> Reset.
+
+  Variables
+    (invariant_overestimator : overestimator (@abstract.invariant _ ap))
+    (guard_decider : overestimator (@abstract.guard _ ap))
+    (reset : vector reset_function n)
+    (reset_components : forall p l l', 
+      pxy (concrete.reset chs l l' p) = 
+      Vmap2 (fun resetF => apply_Reset (resetF l l')) reset (pxy p)).
+
+(*
+  Section disc_trans_regions.
+
+    Variables (eps: Qpos) (l l': concrete.Location chs) (r: abstract.Region ap).
+
+    Definition map_orange' (f: sigT increasing): OpenRange -> OpenRange
+      := let (_, y) := f in map_orange y.
+
+    Definition x_regions :=
+      match reset_x l l' with
+      | Reset_const c => filter (fun r' => overestimate_oranges_overlap eps
+        (* (map_orange' (increasing_const' c) (Xinterval_range (fst r))) (Xinterval_range r')) Xintervals *)
+        (unit_range c: OpenRange) (Xinterval_range r')) Xintervals
+      | Reset_map f => filter (fun r' => overestimate_oranges_overlap eps
+        (map_orange' f (Xinterval_range (fst r))) (Xinterval_range r')) Xintervals
+      | Reset_id => [fst r] (* x reset is id, so we can only remain in this x range *)
+      end.
+
+    Definition y_regions :=
+      match reset_y l l' with
+      | Reset_const c => filter (fun r' => overestimate_oranges_overlap eps
+        (unit_range c: OpenRange) (Yinterval_range r')) Yintervals
+      | Reset_map f => filter (fun r' => overestimate_oranges_overlap eps
+        (map_orange' f (Yinterval_range (snd r))) (Yinterval_range r')) Yintervals
+      | Reset_id => [snd r] (* x reset is id, so we can only remain in this x range *)
+      end.
+
+    Definition disc_trans_regions: list (abstract.Region ap)
+      :=
+      if overestimation_bool (guard_decider l r l') &&
+          overestimation_bool (invariant_overestimator (l, r)) then
+       filter (fun s => overestimation_bool (invariant_overestimator (l', s))) (cart x_regions y_regions)
+     else [].
+
+  End disc_trans_regions.
+
+  Definition raw_disc_trans (eps: Qpos) (s: abstract.State ap): list (abstract.State ap) :=
+    let (l, r) := s in
+    flat_map (fun l' => map (pair l') (disc_trans_regions eps l l' r)) (concrete.locations chs).
+
+  Lemma NoDup_disc_trans eps s: NoDup (raw_disc_trans eps s).
+
+  Hint Resolve in_map_orange.
+
+  Definition is_id_reset (r: Reset): bool :=
+    match r with
+    | Reset_id => true
+    | _ => false
+    end.
+
+  Hint Unfold abstract.invariant abstract.guard.
+
+  Lemma respects_disc (eps: Qpos) (s1 s2 : concrete.State chs):
+    concrete.disc_trans s1 s2 -> forall i1, abstract.in_region ap (snd s1) i1 ->
+    DN (exists i2, abstract.in_region ap (snd s2) i2 /\
+    In (fst s2, i2) (raw_disc_trans eps (fst s1, i1))).
+
+  Program Definition disc_trans: Qpos ->
+    abstract.sharing_transition_overestimator ap (@concrete.disc_trans chs) := raw_disc_trans.
+
+  Program Definition cont_trans_cond_dec eps l r r':
+    overestimation (abstract.cont_trans ap l r r') :=
+      square_flow_conditions.decide_practical
+        (xflow_invr l) (yflow_invr l) (square r) (square r') eps &&
+      invariant_overestimator (l, r) &&
+      invariant_overestimator (l, r').
+*)
+
 End contents.
